backend/Allocproof.v
@@ -2416,28 +2416,58 @@ Proof.
     specialize (NO_CROSS_PTR X).
     (* Seems we could try to conclude using the following assumptions? *)
     (* clear -B1 NO_CROSS_PTR Heqo1 Heqo2. *)
-
-    clear -Heqo2 Hl B1 NO_CROSS_PTR.
+    (* Val.has_type_list rs ## args (sig_args sg) *)
+    assert (Htype_list: Val.has_type_list rs ## args (sig_args sg)).
+    { inv WTI. rewrite <- H10.
+      clear -WTRS. eapply wt_regset_list. eauto. }
+    clear -Heqo2 Hl B1 NO_CROSS_PTR Htype_list.
     eapply add_equations_args_lessdef with (rs := rs) in Heqo2; eauto.
     unfold args' in Heqo2.
     rewrite <- call_regs_param_values in Heqo2.
-    destruct sg. unfold loc_parameters in *. unfold loc_arguments in *.
-    induction sig_args.
-    - simpl in *. contradiction.
-    - simpl in *. destruct a; admit.
-      (* + simpl in *. destruct Hl as [Hl | Hl]. *)
-      (*   * subst. simpl. *)
-      (*     unfold undef_regs. Local Transparent destroyed_at_function_entry. *)
-      (*     unfold destroyed_at_function_entry. *)
-      (*     Local Opaque destroyed_at_function_entry. *)
-      (*     unfold call_regs. *)
-      (*     rewrite Locmap.gso; try congruence. *)
-      (*     inv Heqo2. inv H2. rewrite <- H in NO_CROSS_PTR. inv NO_CROSS_PTR. eauto. *)
-      (*     rewrite <- H in NO_CROSS_PTR. inv NO_CROSS_PTR. inv H2. *)
-      (*   * admit. *)
-      (* + unfold regs_of_rpairs in Hl. *)
-      (*   admit. *)
-    - admit. }
+    pose proof (Val.lessdef_list_not_ptr _ _ Heqo2 NO_CROSS_PTR) as H. clear Heqo2.
+    eapply in_regs_of_rpairs_inv in Hl as [p [H1 H2]].
+    (* assert (H3: In l (map (fun p : rpair loc => Locmap.getpair p (call_regs ls1)) *)
+    (*                     (map (map_rpair parameter_of_argument) (loc_arguments sg)))). *)
+    assert (H3: In (Locmap.getpair p (call_regs ls1))
+                   (map (fun p : rpair loc => Locmap.getpair p (call_regs ls1)) (loc_parameters sg))).
+    (* argument = outgoing  (arguments that are passed to the function that is going to be called)
+       parameter = incoming  (parameters that were passed to the current function)
+     *)
+    { apply in_map with (f := (fun p => Locmap.getpair p (call_regs ls1))). exact H1. }
+    rewrite Forall_forall in H.
+    eapply H in H3.
+    Local Transparent destroyed_at_function_entry.
+    unfold destroyed_at_function_entry. simpl.
+    assert (Loc.diff (R R30) l).
+    { unfold loc_parameters in H1.
+      pose proof (loc_arguments_acceptable) as Haccept.
+      eapply in_map_iff in H1 as [x [? H1]]. subst p.
+      eapply Haccept in H1.
+      destruct x.
+      - simpl in H1.
+        destruct H2 as [H2 | []]. subst l.
+        destruct r as [[] | []]; simpl; try congruence; eauto.
+        simpl in H1; intuition.
+      - simpl in H1.
+        destruct H2 as [H2 | []]; subst.
+        + destruct rhi as [[] | []]; simpl; try congruence; eauto.
+          simpl in H1; intuition.
+        + destruct rlo as [[] | []]; simpl; try congruence; eauto.
+          simpl in H1; intuition.
+        + inv H0. }
+    rewrite Locmap.gso; eauto.
+    destruct p.
+    - simpl in H3, H2. destruct H2; try contradiction; subst r. exact H3.
+    - destruct H2 as [H2 | [H2 | H2]]; try contradiction; subst l.
+      + simpl in *.
+        unfold Val.longofwords in H3.
+        destruct (call_regs ls1 rhi); simpl; auto.
+      + simpl in *.
+        unfold Val.longofwords in H3.
+        destruct (call_regs ls1 rhi);
+          destruct (call_regs ls1 rlo);
+          simpl in *; auto.
+  }
   traceEq. traceEq.
   exploit analyze_successors; eauto. simpl. left; eauto. intros [enext [U V]].
   econstructor; eauto.
@@ -2623,7 +2653,7 @@ Proof.
   eapply plus_left. constructor. eexact A. traceEq.
   econstructor; eauto.
   apply wt_regset_assign; auto. rewrite WTRES0; auto.
-Admitted.
+Qed.
 
 Lemma initial_states_simulation:
   forall st1, RTL.initial_state prog st1 ->
